ironfleet/src/Dafny/Distributed/Impl/Raft/ServerImplNoReceiveClock.i.dfy
@@ -38,7 +38,7 @@ method Server_Next_NoReceive_ReadClock(server_impl:ServerImpl)
   returns (ok:bool, ghost net_event_log:seq<NetEvent>, ghost ios:seq<RaftIo>)
   requires server_impl.nextActionIndex == 1
   requires server_impl.Valid()
-  modifies server_impl.repr
+  modifies server_impl.repr, server_impl.random_generator
   ensures server_impl.repr == old(server_impl.repr)
   ensures server_impl.net_client != null
   ensures ok == NetClientOk(server_impl.net_client)
@@ -60,12 +60,14 @@ method Server_Next_NoReceive_ReadClock(server_impl:ServerImpl)
   ios := [];
 
   if server_impl.nextActionIndex == 1 {
-    var clock,netEvent0 := ReadClock(server_impl.net_client);
-    ghost var io0 := LIoOpReadClock(clock.t as int);
-    ghost var ios_head := [io0];
-    ghost var log_head := [netEvent0];
+    var clock,clock_event := ReadClock(server_impl.net_client);
+    ghost var clock_io := LIoOpReadClock(clock.t as int);
+    ghost var ios_head := [clock_io];
+    ghost var log_head := [clock_event];
     ghost var log_tail := [];
     ghost var ios_tail := [];
+    net_event_log := log_head;
+    ios := ios_head;
     ghost var preDeliveryHistory := server_impl.Env().net.history();
     // Default return
     net_event_log := log_head;
@@ -80,8 +82,9 @@ method Server_Next_NoReceive_ReadClock(server_impl:ServerImpl)
         
         // Create packets
         var outbound_packets:seq<CPacket> := [];
-        ok, outbound_packets := Server_CreateAppendEntriesForAll(server_impl);
+        ok, outbound_packets := Server_CreateAppendEntriesForAll(server_impl, true);
         if (!ok) {
+          print "prepare AppendEntries failed\n";
           ok := true;
           return;
         }
@@ -103,13 +106,40 @@ method Server_Next_NoReceive_ReadClock(server_impl:ServerImpl)
     } else {
       if (clock.t >= server_impl.next_election_time) {
         var const_params := server_impl.config.global_config.params;
-        var next_election_delta := GenerateElectionTimeout(const_params);
+        var next_election_delta := server_impl.random_generator.NextInt(
+          const_params.min_election_timeout,
+          const_params.max_election_timeout
+        );
         var next_election_time := UpperBoundedAdditionImpl(clock.t, next_election_delta, const_params.max_integer_value);
         server_impl.next_election_time := next_election_time;
         if (!ok) { return; }
-        // print "My election timeout!!\n";
-        ios := [io0];
-        net_event_log := [netEvent0];
+        print "My election timeout!!\n";
+        ios := [clock_io];
+        net_event_log := [clock_event];
+        // TODO: need to increase my term
+        if server_impl.current_term > 0xFFFF_FFFF_FFFF_FFFF - 1 {
+          ok := true;
+          return;
+        }
+        server_impl.current_term := server_impl.current_term + 1;
+        server_impl.BecomeCandidate();
+        var outbound_packets;
+        ok, outbound_packets := Server_CreateRequestVoteForAll(server_impl);
+        if (!ok) {
+          ok := true;
+          return;
+        }
+        assert |outbound_packets| <= |server_impl.config.global_config.server_eps| <= 0xFFFF_FFFF_FFFF_FFFF;
+        assert (forall p :: p in outbound_packets ==> CPacketIsSendable(p));
+        ok, log_tail, ios_tail := DeliverOutboundPackets(server_impl, PacketSequence(outbound_packets));
+        if (!ok) { return; }
+        ios := ios_head + ios_tail;
+        net_event_log := log_head + log_tail;
+        assert net_event_log[0].LIoOpReadClock?;
+        assert forall i::0<=i<|log_tail| ==> AbstractifyNetEventToRaftIo(log_tail[i]) == ios_tail[i];
+        assert forall i::0<=i<|log_tail| ==> log_tail[i].LIoOpSend? && ios_tail[i].LIoOpSend?;
+        assert forall i :: 1 <= i < |net_event_log| ==> net_event_log[i].LIoOpSend?;
+        assert forall i :: 0 <= i < |net_event_log| - 1 ==> net_event_log[i].LIoOpReceive? || net_event_log[i+1].LIoOpSend?;
       } else {
         net_event_log := log_head;
         ios := ios_head;
