ironfleet/src/Dafny/Distributed/Impl/Raft/ServerImplProcessPacketX.i.dfy
@@ -107,7 +107,7 @@ method Server_Next_ProcessRequest(server_impl:ServerImpl, ghost old_net_history:
     print "append success!!!\n";
     // Create packets
     var outbound_packets:seq<CPacket> := [];
-    ok, outbound_packets := Server_CreateAppendEntriesForAll(server_impl);
+    ok, outbound_packets := Server_CreateAppendEntriesForAll(server_impl, false);
     if (!ok) {
       ok := true;
       return;
@@ -126,11 +126,11 @@ method Server_Next_ProcessRequest(server_impl:ServerImpl, ghost old_net_history:
   } else {
     var leader_id;
     if (server_impl.current_leader.Some?) {
-      leader_id := GetEndPointIndex(server_impl.config.global_config, server_impl.current_leader.v);
+      leader_id := server_impl.current_leader.v;
     } else {
       leader_id := GetEndPointIndex(server_impl.config.global_config, server_impl.config.server_ep);
     }
-    var msg := CMessage_Reply(recved_msg.seqno_req, 1, leader_id, []);
+    var msg := CMessage_Reply(recved_msg.seqno_req, 0, leader_id, []);
     var packet := CPacket(rr.cpacket.src, server_impl.config.server_ep , msg);
     var outbound_packets := OutboundPacket(Some(packet));
     ok, log_tail, ios_tail := DeliverOutboundPackets(server_impl, outbound_packets);
@@ -149,12 +149,12 @@ method Server_Next_ProcessRequest(server_impl:ServerImpl, ghost old_net_history:
 // Process AppendEntries
 //////////////////////////////////////////////////////////
 method Server_ResetNextElectionTime(server_impl:ServerImpl) returns (ghost clock_event:NetEvent, ghost clock_io:RaftIo)
-  requires server_impl.role == Follower
+  requires server_impl.role == Follower || server_impl.role == Candidate
   requires server_impl.Valid()
   // requires history_after_recv == server_impl.Env().net.history()
-  modifies server_impl, NetClientRepr(server_impl.net_client)
+  modifies server_impl, NetClientRepr(server_impl.net_client), server_impl.random_generator
   ensures clock_event.LIoOpReadClock? && clock_io.LIoOpReadClock?
-  ensures server_impl.role == Follower
+  ensures server_impl.role == old(server_impl.role)
   ensures server_impl.Valid()
   // ensures io and event consistent
   ensures AbstractifyNetEventToRaftIo(clock_event) == clock_io
@@ -170,10 +170,99 @@ method Server_ResetNextElectionTime(server_impl:ServerImpl) returns (ghost clock
   var const_params := server_impl.config.global_config.params;
   var clock;
   clock, clock_event := ReadClock(server_impl.net_client);
-  var election_timeout_delta := GenerateElectionTimeout(const_params);
-  var next_election_time := UpperBoundedAdditionImpl(clock.t, election_timeout_delta, const_params.max_integer_value);
+  var next_election_delta := server_impl.random_generator.NextInt(
+    const_params.min_election_timeout,
+    const_params.max_election_timeout
+  );
+  var next_election_time := UpperBoundedAdditionImpl(clock.t, next_election_delta, const_params.max_integer_value);
   server_impl.next_election_time := next_election_time;
   clock_io := LIoOpReadClock(clock.t as int);
+}
+
+method Server_HandleAppendEntries_TryToAppendAndSend(server_impl:ServerImpl, ghost old_net_history:seq<NetEvent>, rr:ReceiveResult) 
+  returns (ok:bool, ghost net_event_log:seq<NetEvent>, ghost ios:seq<RaftIo>)
+  // About recved things
+  requires rr.RRPacket?
+  requires rr.cpacket.msg.CMessage_AppendEntries?
+  // About server
+  requires server_impl.role == Follower
+  requires server_impl.Valid()
+  requires server_impl.Env().net.history() == old_net_history
+  requires CPacketIsSendable(rr.cpacket)
+  requires ConfigStateIsValid(server_impl.config.global_config)
+  modifies server_impl, server_impl.repr, server_impl.net_client
+  ensures server_impl.repr == old(server_impl.repr)
+  ensures server_impl.net_client != null
+  ensures server_impl.Env().Valid() && server_impl.Env().ok.ok() ==> ok
+  ensures server_impl.Env() == old(server_impl.Env());
+  ensures ok ==> 
+            && server_impl.Valid()
+            && server_impl.nextActionIndex == old(server_impl.nextActionIndex)
+            && AllIosAreSends(ios)
+            // TOPROVE
+            // && (|| Q_RaftServer_Next_ProcessPacket(old(server_impl.AbstractifyToRaftServer()), server_impl.AbstractifyToRaftServer(), ios)
+            //     || (&& IosReflectIgnoringUnsendable(net_event_log)
+            //        && old(server_impl.AbstractifyToRaftServer()) == server_impl.AbstractifyToRaftServer()))
+            && RawIoConsistentWithSpecIO(net_event_log, ios)
+            && OnlySentMarshallableData(net_event_log)
+            && old_net_history + net_event_log == server_impl.Env().net.history()
+            && forall i :: 0 <= i < |net_event_log| - 1 ==> net_event_log[i].LIoOpReceive? || net_event_log[i+1].LIoOpSend?
+{
+  var msg := rr.cpacket.msg;
+  var my_last_log := server_impl.GetLastLogEntry();
+  var success := 0;
+  var match_index := 0;
+  net_event_log := [];
+
+  ios := [];
+  // check whether we can put the entries
+  if msg.prev_log_index > 0xFFFF_FFFF_FFFF_FFFE 
+    && (msg.prev_log_index as int + 1 + |msg.entries| > ServerMaxLogSize())
+  {
+    ok := true;
+    print "[Error] msg.prev_log_index too large";
+    return;
+  }
+  // if |server_impl.log| > 1 {
+  //   var my_last2_log := server_impl.log[|server_impl.log| - 2];
+  //   print "msg.prev_log_index=", msg.prev_log_index, ",msg.prev_log_term=", msg.prev_log_term, ", my_last_log=(index=", my_last_log.index, ",term=", my_last_log.term, "), my_last2_log=(index=", my_last2_log.index, ",term=", my_last2_log.term, ")\n";
+  // } else{
+  //   print "msg.prev_log_index=", msg.prev_log_index, ",msg.prev_log_term=", msg.prev_log_term, ", my_last_log=(index=", my_last_log.index, ",term=", my_last_log.term, ")\n";
+  // }
+
+  var my_log_at_prev_log_index := None;
+  if (msg.prev_log_index <= my_last_log.index) {
+    my_log_at_prev_log_index := server_impl.GetLogEntry(msg.prev_log_index);
+    // TOPROVE: my_log_at_prev_log_index is not None
+  }
+  if (msg.prev_log_index == 0 
+    || (msg.prev_log_index <= my_last_log.index && my_log_at_prev_log_index.Some? && msg.prev_log_term == my_log_at_prev_log_index.v.term)
+  ) {
+    success := 1;
+    assert |msg.entries| > 0 ==> server_impl.log[msg.prev_log_index].index as int + 1 == msg.entries[0].index as int;
+    if |msg.entries| == 0 {
+      match_index := msg.prev_log_index;
+    } else {
+      server_impl.log := server_impl.log[..msg.prev_log_index+1] + msg.entries;
+      match_index := my_last_log.index;
+    }
+    if (msg.leader_commit > server_impl.commit_index) {
+      server_impl.commit_index := msg.leader_commit;
+    }
+    print "After appending, |log|=", |server_impl.log|, "\n";
+  } else {
+    print "Not yet uptodate, cannot append\n";
+  }
+  var send_msg := CMessage_AppendEntriesReply(server_impl.current_term, success, match_index);
+  var send_packet := CPacket(rr.cpacket.src, server_impl.config.server_ep, send_msg);
+  ghost var log_tail, ios_tail;
+  ok, log_tail, ios_tail := DeliverOutboundPackets(server_impl, OutboundPacket(Some(send_packet)));
+  if (!ok) { return; }
+  net_event_log := net_event_log + log_tail;
+  ios := ios + ios_tail;
+  assert forall i::0<=i<|log_tail| ==> AbstractifyNetEventToRaftIo(log_tail[i]) == ios_tail[i];
+  assert forall i::0<=i<|log_tail| ==> log_tail[i].LIoOpSend? && ios_tail[i].LIoOpSend?;
+  assert forall i :: 0 <= i < |net_event_log| - 1 ==> net_event_log[i].LIoOpReceive? || net_event_log[i+1].LIoOpSend?;
 }
 
 method Server_HandleAppendEntries(server_impl:ServerImpl, ghost old_net_history:seq<NetEvent>, rr:ReceiveResult, ghost receive_event:NetEvent) 
@@ -188,7 +277,7 @@ method Server_HandleAppendEntries(server_impl:ServerImpl, ghost old_net_history:
   requires server_impl.Env().net.history() == old_net_history + [receive_event]
   requires CPacketIsSendable(rr.cpacket)
   requires ConfigStateIsValid(server_impl.config.global_config)
-  modifies server_impl, server_impl.repr, server_impl.net_client;
+  modifies server_impl, server_impl.repr, server_impl.net_client, server_impl.random_generator
   ensures server_impl.repr == old(server_impl.repr)
   ensures server_impl.net_client != null
   ensures server_impl.Env().Valid() && server_impl.Env().ok.ok() ==> ok
@@ -207,6 +296,8 @@ method Server_HandleAppendEntries(server_impl:ServerImpl, ghost old_net_history:
 {
   ghost var receive_io := LIoOpReceive(AbstractifyNetPacketToRaftPacket(receive_event.r));
   var msg := rr.cpacket.msg;
+  net_event_log := [receive_event];
+  ios := [receive_io];
 
   var success := 0;
   var match_index := 0;
@@ -217,6 +308,16 @@ method Server_HandleAppendEntries(server_impl:ServerImpl, ghost old_net_history:
   }
   var my_last_log := server_impl.GetLastLogEntry();
   assert server_impl.Valid();
+  // update my leader
+  if (server_impl.current_term == msg.term) {
+    if rr.cpacket.src !in server_impl.config.global_config.server_eps {
+      print "[Error] src not in server_eps\n";
+      ok := true;
+      return;
+    }
+    var src_id := GetEndPointIndex(server_impl.config.global_config, rr.cpacket.src);
+    server_impl.current_leader := Some(src_id);
+  }
   if (server_impl.current_term == msg.term) {
     print "Trying to append #of entries=", |msg.entries|, "\n";
     // Reset role to follower;
@@ -225,46 +326,65 @@ method Server_HandleAppendEntries(server_impl:ServerImpl, ghost old_net_history:
     ghost var clock_event, clock_io := Server_ResetNextElectionTime(server_impl);
     assert my_last_log.index as int == |server_impl.log| - 1;
     assert server_impl.Valid();
-    net_event_log := [receive_event, clock_event];
-    ios := [receive_io, clock_io];
+    net_event_log := net_event_log + [clock_event];
+    ios := ios + [clock_io];
     assert net_event_log[0].LIoOpReceive?;
     assert net_event_log[1].LIoOpReadClock?;
-    // check whether we can put the entries
-    if msg.prev_log_index > 0xFFFF_FFFF_FFFF_FFFE 
-      && (msg.prev_log_index as int + 1 + |msg.entries| > ServerMaxLogSize()
-    ){
-      ok := true;
-      print "[Error] msg.prev_log_index too large";
-      return;
-    }
-    if (msg.prev_log_index == 0 
-      || (msg.prev_log_index <= my_last_log.index && msg.prev_log_term == my_last_log.term)
-    ) {
-      success := 1;
-      assert |msg.entries| > 0 ==> server_impl.log[msg.prev_log_index].index as int + 1 == msg.entries[0].index as int;
-      server_impl.log := server_impl.log[..msg.prev_log_index+1] + msg.entries;
-      if |msg.entries| == 0 {
-        match_index := msg.prev_log_index;
-      } else {
-        match_index := my_last_log.index;
-      }
-      if (msg.leader_commit > server_impl.commit_index) {
-        server_impl.commit_index := msg.leader_commit;
-      }
-      print "After appending, |log|=", |server_impl.log|, "\n";
-    } else {
-      print "Not yet uptodate, cannot append\n";
-    }
-    var send_msg := CMessage_AppendEntriesReply(server_impl.current_term, success, match_index);
-    var send_packet := CPacket(rr.cpacket.src, server_impl.config.server_ep, send_msg);
-    ghost var log_tail, ios_tail;
-    ok, log_tail, ios_tail := DeliverOutboundPackets(server_impl, OutboundPacket(Some(send_packet)));
+    ghost var net_event_log_2:seq<NetEvent> := [];
+    ghost var ios_2:seq<RaftIo> := [];
+    var old_net_history_2 := server_impl.Env().net.history();
+    ok, net_event_log_2, ios_2 := Server_HandleAppendEntries_TryToAppendAndSend(server_impl, old_net_history_2, rr);
+    // net_event_log_2 := [];
+    // ios_2 := [];
+    // ok := true;
     if (!ok) { return; }
-    net_event_log := net_event_log + log_tail;
-    ios := ios + ios_tail;
-    assert forall i::0<=i<|log_tail| ==> AbstractifyNetEventToRaftIo(log_tail[i]) == ios_tail[i];
-    assert forall i::0<=i<|log_tail| ==> log_tail[i].LIoOpSend? && ios_tail[i].LIoOpSend?;
+    net_event_log := net_event_log + net_event_log_2;
+    ios := ios + ios_2;
+    assert forall i::0<=i<|net_event_log_2| ==> AbstractifyNetEventToRaftIo(net_event_log_2[i]) == ios_2[i];
+    assert forall i::0<=i<|net_event_log_2| ==> net_event_log_2[i].LIoOpSend? && ios_2[i].LIoOpSend?;
     assert forall i :: 0 <= i < |net_event_log| - 1 ==> net_event_log[i].LIoOpReceive? || net_event_log[i+1].LIoOpSend?;
+    
+    // check whether we can put the entries
+    // if msg.prev_log_index > 0xFFFF_FFFF_FFFF_FFFE 
+    //   && (msg.prev_log_index as int + 1 + |msg.entries| > ServerMaxLogSize())
+    // {
+    //   ok := true;
+    //   print "[Error] msg.prev_log_index too large";
+    //   return;
+    // }
+    // var my_log_at_prev_log_index := None;
+    // if (msg.prev_log_index <= my_last_log.index) {
+    //   my_log_at_prev_log_index := server_impl.GetLogEntry(msg.prev_log_index);
+    //   // TOPROVE: my_log_at_prev_log_index is not None
+    // }
+    // if (msg.prev_log_index == 0 
+    //   || (msg.prev_log_index <= my_last_log.index && my_log_at_prev_log_index.Some? && msg.prev_log_term == my_log_at_prev_log_index.v.term)
+    // ) {
+    //   success := 1;
+    //   assert |msg.entries| > 0 ==> server_impl.log[msg.prev_log_index].index as int + 1 == msg.entries[0].index as int;
+    //   if |msg.entries| == 0 {
+    //     match_index := msg.prev_log_index;
+    //   } else {
+    //     server_impl.log := server_impl.log[..msg.prev_log_index+1] + msg.entries;
+    //     match_index := my_last_log.index;
+    //   }
+    //   if (msg.leader_commit > server_impl.commit_index) {
+    //     server_impl.commit_index := msg.leader_commit;
+    //   }
+    //   print "After appending, |log|=", |server_impl.log|, "\n";
+    // } else {
+    //   print "Not yet uptodate, cannot append\n";
+    // }
+    // var send_msg := CMessage_AppendEntriesReply(server_impl.current_term, success, match_index);
+    // var send_packet := CPacket(rr.cpacket.src, server_impl.config.server_ep, send_msg);
+    // ghost var log_tail, ios_tail;
+    // ok, log_tail, ios_tail := DeliverOutboundPackets(server_impl, OutboundPacket(Some(send_packet)));
+    // if (!ok) { return; }
+    // net_event_log := net_event_log + log_tail;
+    // ios := ios + ios_tail;
+    // assert forall i::0<=i<|log_tail| ==> AbstractifyNetEventToRaftIo(log_tail[i]) == ios_tail[i];
+    // assert forall i::0<=i<|log_tail| ==> log_tail[i].LIoOpSend? && ios_tail[i].LIoOpSend?;
+    // assert forall i :: 0 <= i < |net_event_log| - 1 ==> net_event_log[i].LIoOpReceive? || net_event_log[i+1].LIoOpSend?;
   } else {
     net_event_log := [receive_event];
     ios := [receive_io];
@@ -328,12 +448,6 @@ method Server_HandleAppendEntriesReply(server_impl:ServerImpl, ghost old_net_his
 
   if (server_impl.role == Leader && server_impl.current_term == msg.term) {
     if (msg.success == 1) {
-      assert forall ep :: ep in server_impl.config.global_config.server_eps ==> (
-        && ep in server_impl.next_index 
-        && ep in server_impl.match_index
-        && 1 <= server_impl.next_index[ep] <= |server_impl.log| as uint64
-        && 0 <= server_impl.match_index[ep] < server_impl.next_index[ep]
-      );
       if (msg.match_index > MaxLogEntryIndex() as uint64 - 1) {
         print "[Error] match_index too large\n";
         return;
@@ -357,16 +471,188 @@ method Server_HandleAppendEntriesReply(server_impl:ServerImpl, ghost old_net_his
       }
     } else {
       var decreased_index;
-      if server_impl.next_index[ep] > 1 {
-        decreased_index := server_impl.next_index[ep];
+      if server_impl.next_index[ep] > LogEntrySeqSizeLimit() as uint64 {
+        decreased_index := server_impl.next_index[ep] - LogEntrySeqSizeLimit() as uint64;
       } else {
         decreased_index := 1;
       }
+      server_impl.match_index := server_impl.match_index[ep := 0];
       server_impl.next_index := server_impl.next_index[ep := decreased_index];
     }
   }
 
 }
+
+//////////////////////////////////////////////////////////
+// Process RequestVote
+//////////////////////////////////////////////////////////
+method Server_HandleReqeustVote(server_impl:ServerImpl, ghost old_net_history:seq<NetEvent>, rr:ReceiveResult, ghost receive_event:NetEvent) 
+  returns (ok:bool, ghost net_event_log:seq<NetEvent>, ghost ios:seq<RaftIo>)
+  // About recved things
+  requires receive_event.LIoOpReceive?
+  requires rr.RRPacket?
+  requires NetPacketIsAbstractable(receive_event.r)
+  requires rr.cpacket.msg.CMessage_RequestVote?
+  // About server
+  requires server_impl.Valid()
+  requires server_impl.Env().net.history() == old_net_history + [receive_event]
+  requires CPacketIsSendable(rr.cpacket)
+  requires ConfigStateIsValid(server_impl.config.global_config)
+  modifies server_impl, server_impl.repr, server_impl.net_client, server_impl.random_generator
+  ensures server_impl.repr == old(server_impl.repr)
+  ensures server_impl.net_client != null
+  ensures server_impl.Env().Valid() && server_impl.Env().ok.ok() ==> ok
+  ensures server_impl.Env() == old(server_impl.Env());
+  ensures ok ==> 
+            && server_impl.Valid()
+            && server_impl.nextActionIndex == old(server_impl.nextActionIndex)
+            // PROVE
+            // && (|| Q_RaftServer_Next_ProcessPacket(old(server_impl.AbstractifyToRaftServer()), server_impl.AbstractifyToRaftServer(), ios)
+            //     || (&& IosReflectIgnoringUnsendable(net_event_log)
+            //        && old(server_impl.AbstractifyToRaftServer()) == server_impl.AbstractifyToRaftServer()))
+            && RawIoConsistentWithSpecIO(net_event_log, ios)
+            && OnlySentMarshallableData(net_event_log)
+            && old_net_history + net_event_log == server_impl.Env().net.history()
+            && forall i :: 0 <= i < |net_event_log| - 1 ==> net_event_log[i].LIoOpReceive? || net_event_log[i+1].LIoOpSend?
+{
+  ghost var receive_io := LIoOpReceive(AbstractifyNetPacketToRaftPacket(receive_event.r));
+  var msg := rr.cpacket.msg;
+  // setup default return values
+  net_event_log := [receive_event];
+  ios := [receive_io];
+  ok := true;
+
+  var granted := 0;
+  if (server_impl.current_term < msg.term) {
+    server_impl.current_term := msg.term;
+    server_impl.voted_for := None;
+    server_impl.role := Follower;
+  }
+
+  if (server_impl.role == Leader || server_impl.role == Candidate) {
+    return;
+  }
+
+  var my_last_log := server_impl.GetLastLogEntry();
+  if (
+    server_impl.current_term == msg.term
+    && (server_impl.voted_for == None || server_impl.voted_for == Some(msg.candidate_id))
+    && (msg.last_log_term > my_last_log.term || (msg.last_log_term == my_last_log.term && msg.last_log_index >= my_last_log.index))
+  ){
+    granted := 1;
+    // reset election timeout before we do any change to server (to avoid proof)
+    ghost var clock_event, clock_io := Server_ResetNextElectionTime(server_impl);
+    assert my_last_log.index as int == |server_impl.log| - 1;
+    assert server_impl.Valid();
+    net_event_log := [receive_event, clock_event];
+    ios := [receive_io, clock_io];
+    assert net_event_log[0].LIoOpReceive?;
+    assert net_event_log[1].LIoOpReadClock?;
+    // update voted_for
+    if (msg.candidate_id >= |server_impl.config.global_config.server_eps| as uint64) {
+      if |server_impl.config.global_config.server_eps| == 3 {
+        print server_impl.config.global_config.server_eps[0], "\n";
+        print server_impl.config.global_config.server_eps[1], "\n";
+        print server_impl.config.global_config.server_eps[2], "\n";
+      }
+      print "[Error] candidate_id(", msg.candidate_id, ") not in cluster\n";
+      return;
+    }
+    server_impl.voted_for := Some(msg.candidate_id);
+    server_impl.current_leader := Some(msg.candidate_id);
+  }
+  // send reply
+  var reply_msg := CMessage_RequestVoteReply(server_impl.current_term, granted);
+  var reply_packet := CPacket(rr.cpacket.src, server_impl.config.server_ep, reply_msg);
+  ghost var log_tail, ios_tail;
+  ok, log_tail, ios_tail := DeliverOutboundPackets(server_impl, OutboundPacket(Some(reply_packet)));
+  if (!ok) { return; }
+  net_event_log := net_event_log + log_tail;
+  ios := ios + ios_tail;
+  assert forall i::0<=i<|log_tail| ==> AbstractifyNetEventToRaftIo(log_tail[i]) == ios_tail[i];
+  assert forall i::0<=i<|log_tail| ==> log_tail[i].LIoOpSend? && ios_tail[i].LIoOpSend?;
+  assert forall i :: 0 <= i < |net_event_log| - 1 ==> net_event_log[i].LIoOpReceive? || net_event_log[i+1].LIoOpSend?;
+}
+
+//////////////////////////////////////////////////////////
+// Process RequestVoteReply
+//////////////////////////////////////////////////////////
+method Server_HandleReqeustVoteReply(server_impl:ServerImpl, ghost old_net_history:seq<NetEvent>, rr:ReceiveResult, ghost receive_event:NetEvent) 
+  returns (ok:bool, ghost net_event_log:seq<NetEvent>, ghost ios:seq<RaftIo>)
+  // About recved things
+  requires receive_event.LIoOpReceive?
+  requires rr.RRPacket?
+  requires NetPacketIsAbstractable(receive_event.r)
+  requires rr.cpacket.msg.CMessage_RequestVoteReply?
+  // About server
+  requires server_impl.Valid()
+  requires server_impl.Env().net.history() == old_net_history + [receive_event]
+  requires CPacketIsSendable(rr.cpacket)
+  requires ConfigStateIsValid(server_impl.config.global_config)
+  modifies server_impl, server_impl.repr, server_impl.net_client
+  ensures server_impl.repr == old(server_impl.repr)
+  ensures server_impl.net_client != null
+  ensures server_impl.Env().Valid() && server_impl.Env().ok.ok() ==> ok
+  ensures server_impl.Env() == old(server_impl.Env());
+  ensures ok ==> 
+            && server_impl.Valid()
+            && server_impl.nextActionIndex == old(server_impl.nextActionIndex)
+            // PROVE
+            // && (|| Q_RaftServer_Next_ProcessPacket(old(server_impl.AbstractifyToRaftServer()), server_impl.AbstractifyToRaftServer(), ios)
+            //     || (&& IosReflectIgnoringUnsendable(net_event_log)
+            //        && old(server_impl.AbstractifyToRaftServer()) == server_impl.AbstractifyToRaftServer()))
+            && RawIoConsistentWithSpecIO(net_event_log, ios)
+            && OnlySentMarshallableData(net_event_log)
+            && old_net_history + net_event_log == server_impl.Env().net.history()
+            && forall i :: 0 <= i < |net_event_log| - 1 ==> net_event_log[i].LIoOpReceive? || net_event_log[i+1].LIoOpSend?
+{
+  ghost var receive_io := LIoOpReceive(AbstractifyNetPacketToRaftPacket(receive_event.r));
+  var msg := rr.cpacket.msg;
+  // setup default return values
+  ghost var ios_tail := [];
+  ghost var log_tail := [];
+  net_event_log := [receive_event];
+  ios := [receive_io];
+  ok := true;
+
+  if (server_impl.current_term < msg.term) {
+    server_impl.current_term := msg.term;
+    server_impl.voted_for := None;
+    server_impl.role := Follower;
+  }
+
+  if (server_impl.role == Candidate && server_impl.current_term == msg.term) {
+    // Record the vote
+    server_impl.vote_granted := server_impl.vote_granted[rr.cpacket.src := msg.vote_granted];
+    // Check for step up
+    var passed:bool := server_impl.VoteRequestPassed();
+    print "passed=", passed, "\n";
+    if (passed) {
+      print "election passed, become leader\n";
+      server_impl.BecomeLeader();
+      // Create packets
+      var outbound_packets:seq<CPacket> := [];
+      ok, outbound_packets := Server_CreateAppendEntriesForAll(server_impl, true);
+      if (!ok) {
+        print "prepare AppendEntries failed\n";
+        ok := true;
+        return;
+      }
+      assert |outbound_packets| <= |server_impl.config.global_config.server_eps| <= 0xFFFF_FFFF_FFFF_FFFF;
+      assert (forall p :: p in outbound_packets ==> CPacketIsSendable(p));
+      ok, log_tail, ios_tail := DeliverOutboundPackets(server_impl, PacketSequence(outbound_packets));
+      if (!ok) { return; }
+      ios := ios + ios_tail;
+      net_event_log := net_event_log + log_tail;
+      // print "I broadcast heartbeat!\n";
+      assert forall i::0<=i<|log_tail| ==> AbstractifyNetEventToRaftIo(log_tail[i]) == ios_tail[i];
+      assert forall i::0<=i<|log_tail| ==> log_tail[i].LIoOpSend? && ios_tail[i].LIoOpSend?;
+      assert forall i :: 1 <= i < |net_event_log| ==> net_event_log[i].LIoOpSend?;
+      assert forall i :: 0 <= i < |net_event_log| - 1 ==> net_event_log[i].LIoOpReceive? || net_event_log[i+1].LIoOpSend?;
+    }
+  }
+}
+
 
 //////////////////////////////////////////////////////////
 // Process All Packet.
@@ -375,11 +661,11 @@ method Server_Next_ProcessPacketX(server_impl:ServerImpl)
   returns (ok:bool, ghost net_event_log:seq<NetEvent>, ghost ios:seq<RaftIo>)
   requires server_impl.Valid()
   requires ConfigStateIsValid(server_impl.config.global_config)
-  modifies server_impl, server_impl.repr, server_impl.net_client;
+  modifies server_impl, server_impl.repr, server_impl.net_client, server_impl.random_generator
   ensures server_impl.repr == old(server_impl.repr)
   ensures server_impl.net_client != null
   ensures server_impl.Env().Valid() && server_impl.Env().ok.ok() ==> ok
-  ensures server_impl.Env() == old(server_impl.Env());
+  ensures server_impl.Env() == old(server_impl.Env())
   ensures ok ==> 
             && server_impl.Valid()
             && server_impl.nextActionIndex == old(server_impl.nextActionIndex)
@@ -421,7 +707,7 @@ method Server_Next_ProcessPacketX(server_impl:ServerImpl)
     var msg := rr.cpacket.msg;
     if (msg.CMessage_Request? || msg.CMessage_Reply?) {
       if (msg.CMessage_Request?) {
-        print "server ", my_idx, "(is_leader=", server_impl.role.Leader?, ") received a request(", msg.seqno_req, ", ", msg.req, ")\n";
+        print "server ", my_idx, "(", server_impl.current_term, ",is_leader=", server_impl.role.Leader?, ") received a request(", msg.seqno_req, ", ", msg.req, ")\n";
         ok, net_event_log, ios := Server_Next_ProcessRequest(server_impl, old_net_history, rr, receive_event);
       } else {
         return;
@@ -433,22 +719,29 @@ method Server_Next_ProcessPacketX(server_impl:ServerImpl)
         return;
       }
       var src_id := GetEndPointIndex(server_impl.config.global_config, rr.cpacket.src);
+      // process the message
       if (msg.CMessage_AppendEntries?) {
         // ignore packet from self
         if (rr.cpacket.src == server_impl.config.server_ep) {
           return;
         }
-        print "server ", my_idx, "(is_leader=", server_impl.role.Leader?, 
-          ") received AppendEntries(|entries|=", |msg.entries|, ",prev_log_index=", msg.prev_log_index, ")\n";
+        print "server ", my_idx, "(", server_impl.current_term, ",is_leader=", server_impl.role.Leader?, ",leader=", if server_impl.current_leader.Some? then server_impl.current_leader.v else 0xFFFF_FFFF_FFFF_FFFF, 
+          ") received from ", src_id, "AppendEntries(|entries|=", |msg.entries|, ",prev_log_index=", msg.prev_log_index, ")\n";
         ok, net_event_log, ios := Server_HandleAppendEntries(server_impl, old_net_history, rr, receive_event);
       } else if (msg.CMessage_AppendEntriesReply?) {
         if (server_impl.role != Leader) {
           return;
         }
-        print "server ", my_idx, "(is_leader=", server_impl.role.Leader?, 
-          ") received from ", src_id, " AppendEntriesReply(term=", msg.term, ",success=", msg.success, "match_index=", msg.match_index, ")\n";
+        print "server ", my_idx, "(", server_impl.current_term, ",is_leader=", server_impl.role.Leader?, ",leader=", if server_impl.current_leader.Some? then server_impl.current_leader.v else 0xFFFF_FFFF_FFFF_FFFF, 
+          ") received from ", src_id, " AppendEntriesReply(term=", msg.term, ",success=", msg.success, ",match_index=", msg.match_index, ",commit=", server_impl.commit_index, ")\n";
         ok, net_event_log, ios := Server_HandleAppendEntriesReply(server_impl, old_net_history, rr, receive_event);
+      } else if (msg.CMessage_RequestVote?) {
+        print "server ", my_idx, "(", server_impl.current_term, ",is_leader=", server_impl.role.Leader?, ",leader=", if server_impl.current_leader.Some? then server_impl.current_leader.v else 0xFFFF_FFFF_FFFF_FFFF, ",commit=", server_impl.commit_index, ") received from ", src_id, " RequestVote(term=", msg.term, ")\n";
+        ok, net_event_log, ios := Server_HandleReqeustVote(server_impl, old_net_history, rr, receive_event); 
       } else {
+        assert msg.CMessage_RequestVoteReply?;
+        print "server ", my_idx, "(", server_impl.current_term, ",is_leader=", server_impl.role.Leader?, ",leader=", if server_impl.current_leader.Some? then server_impl.current_leader.v else 0xFFFF_FFFF_FFFF_FFFF, ") received from ", src_id, " RequestVoteReply(term=", msg.term, ",granted=", msg.vote_granted, ")\n";
+        ok, net_event_log, ios := Server_HandleReqeustVoteReply(server_impl, old_net_history, rr, receive_event);
         return;
       }
     }
