ironfleet/weekly_summary/week4.md
@@ -1,0 +1,16 @@
+#### Last Week
+
+- Complete the election part; And now we can run a Raft cluster.
+
+#### This Week Plan
+
+- Complete the `protocol` part
+  - The difference between protocol and implementation
+    - Protocol doesn't contains send/recv details; only need to specify sent/received packets (without marshalling/demarshalling)
+    - Protocol only need to specify the `predicate`s that each actions should hold (including `requires` and `predicate` itself)
+- Prove refinement from `implementation` to `protocol` (shall be easier because they are basically one-to-one corresponding)
+- Prove refinement from `protocol` to `service`
+
+#### Problems
+
+- For `protocol` -> `service`, where to start?
